Weidenbach_Book/IsaSAT_Propagate_Conflict.thy
@@ -5,18 +5,12 @@ begin
 definition (in -) shorten_take_ll where
   \<open>shorten_take_ll L j W = W[L := take j (W ! L)]\<close>
 
-term "Array.update W L (a, j) "
-term "do {
-      (a, n) \<leftarrow> Array.nth W L;
-      d a b
-    }"
 definition (in -) shorten_take_aa where
   \<open>shorten_take_aa L j W =  do {
       (a, n) \<leftarrow> Array.nth W L;
       Array.upd L (a, j) W  
     }\<close>
 
-find_theorems nth_u
 definition (in -) shorten_take_aa_u32 where
   \<open>shorten_take_aa_u32 L j W =  do {
       (a, n) \<leftarrow> nth_u_code W L;
@@ -219,6 +213,7 @@ context isasat_input_bounded_nempty
 begin
 
 (* TODO most of the unfolding should move to the definition *)
+sepref_register isa_find_unwatched_wl_st_heur
 sepref_thm find_unwatched_wl_st_heur_code
   is \<open>uncurry ((PR_CONST isa_find_unwatched_wl_st_heur))\<close>
   :: \<open>[find_unwatched_wl_st_heur_pre]\<^sub>a
@@ -226,7 +221,7 @@ sepref_thm find_unwatched_wl_st_heur_code
   supply [[goals_limit = 1]]
     fmap_length_rll_def[simp] fmap_length_rll_u64_def[simp]
   unfolding isa_find_unwatched_wl_st_heur_def isasat_assn_def PR_CONST_def
-  find_unwatched_def fmap_rll_def[symmetric] fmap_length_rll_u64_def[symmetric]
+  find_unwatched_def fmap_rll_def[symmetric]
   length_u_def[symmetric] isa_find_unwatched_def
   case_tri_bool_If find_unwatched_wl_st_heur_pre_def
   fmap_rll_u64_def[symmetric]
@@ -239,9 +234,9 @@ concrete_definition (in -) find_unwatched_wl_st_heur_code
 prepare_code_thms (in -) find_unwatched_wl_st_heur_code_def
 
 lemmas find_unwatched_wl_st_heur_code_find_unwatched_wl_st_heur[sepref_fr_rules] =
-   find_unwatched_wl_st_heur_code.refine[of \<A>\<^sub>i\<^sub>n, OF isasat_input_bounded_nempty_axioms,
-     unfolded PR_CONST_def]
+   find_unwatched_wl_st_heur_code.refine[of \<A>\<^sub>i\<^sub>n, OF isasat_input_bounded_nempty_axioms]
 
+(* 
 sepref_thm find_unwatched_wl_st_heur_fast_code
   is \<open>uncurry ((PR_CONST find_unwatched_wl_st_heur))\<close>
   :: \<open>[find_unwatched_wl_st_heur_pre]\<^sub>a
@@ -255,7 +250,7 @@ sepref_thm find_unwatched_wl_st_heur_fast_code
   two_uint64_nat_def[symmetric]
   fmap_rll_u64_def[symmetric]
   one_uint64_nat_def[symmetric]
-  by sepref
+  by sepref 
 
 concrete_definition (in -) find_unwatched_wl_st_heur_fast_code
    uses isasat_input_bounded_nempty.find_unwatched_wl_st_heur_fast_code.refine_raw
@@ -266,14 +261,15 @@ prepare_code_thms (in -) find_unwatched_wl_st_heur_fast_code_def
 lemmas find_unwatched_wl_st_heur_code_find_unwatched_wl_st_fast_heur[sepref_fr_rules] =
    find_unwatched_wl_st_heur_fast_code.refine[of \<A>\<^sub>i\<^sub>n, OF isasat_input_bounded_nempty_axioms,
      unfolded PR_CONST_def]
-
+*)
+sepref_register isa_set_lookup_conflict_aa set_conflict_wl_heur
 sepref_thm set_conflict_wl_heur_code
-  is \<open>uncurry set_conflict_wl_heur\<close>
+  is \<open>uncurry (PR_CONST set_conflict_wl_heur)\<close>
   :: \<open>[set_conflict_wl_heur_pre]\<^sub>a
     nat_assn\<^sup>k *\<^sub>a isasat_assn\<^sup>d \<rightarrow> isasat_assn\<close>
   supply [[goals_limit=1]]
   unfolding set_conflict_wl_heur_def isasat_assn_def IICF_List_Mset.lms_fold_custom_empty
-    set_conflict_wl_heur_pre_def
+    set_conflict_wl_heur_pre_def PR_CONST_def
   by sepref
 
 concrete_definition (in -) set_conflict_wl_heur_code
@@ -286,7 +282,7 @@ lemmas set_conflict_wl_heur_code[sepref_fr_rules] =
   set_conflict_wl_heur_code.refine[OF isasat_input_bounded_nempty_axioms]
 
 
-sepref_thm set_conflict_wl_heur_fast_code
+(* sepref_thm set_conflict_wl_heur_fast_code
   is \<open>uncurry set_conflict_wl_heur\<close>
   :: \<open>[set_conflict_wl_heur_pre]\<^sub>a
     uint32_nat_assn\<^sup>k *\<^sub>a isasat_fast_assn\<^sup>d \<rightarrow> isasat_fast_assn\<close>
@@ -302,12 +298,14 @@ concrete_definition (in -) set_conflict_wl_heur_fast_code
 prepare_code_thms (in -) set_conflict_wl_heur_fast_code_def
 
 lemmas set_conflict_wl_heur_fast_code[sepref_fr_rules] =
-  set_conflict_wl_heur_fast_code.refine[OF isasat_input_bounded_nempty_axioms]
+  set_conflict_wl_heur_fast_code.refine[OF isasat_input_bounded_nempty_axioms] *)
 
+find_theorems swap_lits
+sepref_register update_clause_wl_heur
 sepref_thm update_clause_wl_code
-  is \<open>uncurry6 update_clause_wl_heur\<close>
+  is \<open>uncurry6 (PR_CONST update_clause_wl_heur)\<close>
   :: \<open>[update_clause_wl_code_pre]\<^sub>a
-     unat_lit_assn\<^sup>k *\<^sub>a nat_assn\<^sup>k *\<^sub>a nat_assn\<^sup>k *\<^sub>a nat_assn\<^sup>k *\<^sub>a uint64_nat_assn\<^sup>k *\<^sub>a uint64_nat_assn\<^sup>k *\<^sub>a isasat_assn\<^sup>d \<rightarrow>
+     unat_lit_assn\<^sup>k *\<^sub>a nat_assn\<^sup>k *\<^sub>a nat_assn\<^sup>k *\<^sub>a nat_assn\<^sup>k *\<^sub>a nat_assn\<^sup>k *\<^sub>a nat_assn\<^sup>k *\<^sub>a isasat_assn\<^sup>d \<rightarrow>
        nat_assn *a nat_assn *a isasat_assn\<close>
   supply [[goals_limit=1]] length_rll_def[simp] length_ll_def[simp]
   unfolding update_clause_wl_heur_def isasat_assn_def Array_List_Array.swap_ll_def[symmetric]
@@ -317,6 +315,12 @@ sepref_thm update_clause_wl_code
     fmap_rll_u64_def[symmetric]
     fmap_swap_ll_u64_def[symmetric]
     fmap_swap_ll_def[symmetric]
+    PR_CONST_def
+    apply sepref_dbg_keep
+    apply sepref_dbg_trans_keep
+    apply sepref_dbg_trans_step_keep
+    oops
+    apply sepref_dbg_side_unfold apply (auto simp: )[]
   by sepref
 
 concrete_definition (in -) update_clause_wl_code
